Progress on data-cost examples

examples/cost/divProgScript.sml
@@ -2,15 +2,20 @@
   Preliminary data-cost examples
 *)
 
-open preamble basis compilationLib dataSemTheory data_monadTheory;
+open preamble basis compilationLib ;
+open dataSemTheory data_monadTheory dataLangTheory;
 
 val _ = new_theory "divProg"
+
+(* *********************** *)
+(* * Auxiliary functions * *)
+(* *********************** *)
 
 fun to_data prog name =
   let
     val heap_size      = 1000
     val stack_size     = 1000
-    val prog_def       = REFL (process_topdecs prog)
+    val prog_def       = REFL prog
     val cs             = compilation_compset()
     val conf_def       = x64_backend_config_def
     val data_prog_name = name ^ "_data_prog"
@@ -22,21 +27,210 @@ fun to_data prog name =
     (* code *)
     val code      = ``fromAList ^(rhs (concl data_prog_def))``
     val code_name = mk_var (name ^ "_data_code", type_of code)
-    val code_def  = Define `^code_name = ^code`
+    val code_def  = zDefine `^code_name = ^code`
     (* initial call *)
     val initial_call = (rhs o concl o EVAL)
       ``dataLang$Call NONE (SOME ^(conf).clos_conf.start) [] NONE``
     val initial_call_name = mk_var (name ^ "_data_call", type_of initial_call)
     val initial_call_def  = Define `^initial_call_name = ^initial_call`
   in
-    (initial_call,code)
+    (initial_call,code_def)
   end
 
-val pureLoop =
+fun diff_code code1 code2 = let
+  val l1 = code1
+           |> concl                |> rhs
+           |> dest_comb            |> snd
+           |> listSyntax.dest_list |> fst;
+  val l2 = code2
+           |> concl                |> rhs
+           |> dest_comb            |> snd
+           |> listSyntax.dest_list |> fst;
+  val [(p1,p2)] = filter (not o (uncurry aconv)) (zip l1 l2)
+  in (p1,p2)
+  end
+
+fun diff_codes code1 code2 = let
+  val l1 = code1
+           |> concl                |> rhs
+           |> dest_comb            |> snd
+           |> listSyntax.dest_list |> fst;
+  val l2 = code2
+           |> concl                |> rhs
+           |> dest_comb            |> snd
+           |> listSyntax.dest_list |> fst;
+  in filter (not o (uncurry aconv)) (zip l1 l2)
+  end
+
+val _ = translation_extends "basisProg";
+
+val whole_prog = get_ml_prog_state ()
+  |> ml_progLib.clean_state
+  |> ml_progLib.remove_snocs
+  |> ml_progLib.get_prog
+
+Overload monad_unitbind[local] = ``bind``
+Overload return[local] = ``return``
+
+val _ = monadsyntax.temp_add_monadsyntax()
+
+Theorem EVERY_lookup:
+  ∀t. EVERY (\(k,v). lookup k t = SOME v) (toAList t)
+Proof
+  fs [EVERY_MEM,MEM_toAList,FORALL_PROD]
+QED
+
+(* MOVE: sptreeTheory *)
+Theorem domain_IS_SOME:
+  ∀t k. k ∈ domain t = IS_SOME (lookup k t)
+Proof
+  rw [domain_lookup,IS_SOME_EXISTS]
+QED
+
+(* REMOVE *)
+val _ = computeLib.add_thms [size_of_def] computeLib.the_compset;
+
+val _ = sptreeSyntax.temp_add_sptree_printer ()
+
+(* *********** *)
+(* * Tactics * *)
+(* *********** *)
+
+(* Conversion with memoization  *)
+fun mem_conv c =
+  let val memory = ref ([] : (term * thm) list)
+  in fn t => (snd (first (aconv t o fst) (!memory)))
+             handle HOL_ERR _ =>
+                    let val th = QCONV c t
+                    in memory := (t,th) :: (!memory);
+                       th
+                    end
+  end
+
+(* Evaluate a subterm of the goal *)
+fun eval_goalsub_tac pat (asms,goal) =
+   let
+   val tm = goal |> find_term (can (match_term pat))
+   val th = EVAL tm
+   in PURE_ONCE_REWRITE_TAC [th] (asms,goal)
+   end
+
+(* Generate all possible lookup for a code sptree *)
+fun mk_code_lookup code_tm code_def = EVERY_lookup
+    |> Q.ISPEC code_tm
+    |> CONV_RULE ((RAND_CONV o RAND_CONV) (fn tm => code_def))
+    |> CONV_RULE (RAND_CONV EVAL)
+    |> SIMP_RULE (srw_ss()) []
+
+(* remove makespace bindings *)
+val strip_makespace =
+  qmatch_goalsub_abbrev_tac `bind _ rest_mkspc _`
+  \\ REWRITE_TAC [ bind_def, makespace_def ]
+  \\ eval_goalsub_tac ``cut_env _ _`` \\ simp []
+  \\ eval_goalsub_tac ``state_locals_fupd _ _``
+  \\ Q.UNABBREV_TAC `rest_mkspc`
+
+fun mk_strip_assign code_lookup =
+  qmatch_goalsub_abbrev_tac `bind _ rest_ass _`
+  \\ REWRITE_TAC [ bind_def           , assign_def
+                 , op_space_reset_def , closLangTheory.op_case_def
+                 , cut_state_opt_def  , option_case_def
+                 , do_app_def         , data_spaceTheory.op_space_req_def
+                 , do_space_def       , closLangTheory.op_distinct
+                 , MEM                , IS_NONE_DEF
+                 , bvi_to_dataTheory.op_requires_names_eqn ]
+  \\ BETA_TAC
+  \\ TRY(eval_goalsub_tac ``cut_state _ _`` \\ simp [])
+  \\ TRY(eval_goalsub_tac ``get_vars    _ _`` \\ simp [])
+  \\ simp [ do_app_aux_def    , set_var_def    , lookup_def
+          , domain_IS_SOME    , code_lookup    , size_of_heap_def
+          , consume_space_def , with_fresh_ts_def
+          , backend_commonTheory.small_enough_int_def ]
+  \\ eval_goalsub_tac ``state_locals_fupd _ _``
+  \\ Q.UNABBREV_TAC `rest_ass`
+
+fun mk_open_tailcall code_lookup =
+  ASM_REWRITE_TAC [ tailcall_def , find_code_def
+                  , get_vars_def , get_var_def
+                  , lookup_def   , timeout_def ]
+  \\ simp [code_lookup,lookup_def]
+  \\ IF_CASES_TAC >- (simp [data_safe_def,size_of_def] \\ EVAL_TAC)
+  \\ REWRITE_TAC [ call_env_def   , dec_clock_def
+                 , to_shallow_thm , to_shallow_def ]
+  \\ eval_goalsub_tac ``state_locals_fupd _ _``
+
+val close_tailcall =
+  ho_match_mp_tac data_safe_res
+  \\ reverse conj_tac >- (rw [] \\ pairarg_tac \\ rw [])
+
+fun mk_make_tailcall open_tailcall =
+  open_tailcall \\ close_tailcall
+
+fun mk_open_call code_lookup =
+  ASM_REWRITE_TAC [ call_def     , find_code_def , push_env_def
+                  , get_vars_def , call_env_def  , dec_clock_def
+                  , cut_env_def  , domain_def    , data_safe_def
+                  , EMPTY_SUBSET , get_var_def ]
+  \\ simp [code_lookup,lookup_def,domain_IS_SOME]
+  \\ IF_CASES_TAC >- (simp [data_safe_def,size_of_def] \\ EVAL_TAC)
+  \\ REWRITE_TAC [ push_env_def , to_shallow_def , to_shallow_thm]
+  \\ eval_goalsub_tac ``state_locals_fupd _ _``
+
+val close_call =
+  qmatch_goalsub_abbrev_tac `f (state_locals_fupd _ _)`
+  \\ qmatch_goalsub_abbrev_tac `f s`
+  \\ `data_safe (f s)` suffices_by
+     (EVERY_CASE_TAC \\ rw [data_safe_def]
+     \\ fs [data_safe_def,data_safe_move
+           ,set_var_safe_for_space]
+     \\ drule_then drule pop_env_safe_for_space
+     \\ fs [set_var_safe_for_space])
+  \\ Q.UNABBREV_TAC `f`
+  \\ Q.UNABBREV_TAC `s`
+
+fun mk_make_call open_call =
+  open_call \\ close_call
+
+(* val (asms,goal) = top_goal() *)
+
+fun mk_strip_call open_call (asms,goal) =
+  let val free_names = map (fn tm => fst (dest_var tm)) (free_varsl (goal::asms))
+      fun next_name n name =
+          let val new_name = name^"_"^(Int.toString n)
+          in if n = 0
+             then if mem name free_names
+                  then next_name (n+1) name
+                  else [QUOTE name]
+             else if mem new_name free_names
+             then next_name (n+1) name
+             else [QUOTE new_name]
+          end
+  in (qmatch_goalsub_abbrev_tac (`bind _ ` @ (next_name 0 "rest_call") @ ` _`)
+     \\ ONCE_REWRITE_TAC [bind_def]
+     \\ open_call \\ rw [data_safe_def]) (asms,goal)
+  end
+
+val make_if =
+  simp [if_var_def,data_safe_def,lookup_def]
+  \\ REWRITE_TAC [ isBool_def
+                 , backend_commonTheory.bool_to_tag_def
+                 , backend_commonTheory.true_tag_def
+                 , backend_commonTheory.false_tag_def]
+  \\ simp [pop_env_def]
+  \\ eval_goalsub_tac ``state_locals_fupd _ _``
+
+
+(* ************ *)
+(* * pureLoop * *)
+(* ************ *)
+
+(* A simple infinite loop that does nothing *)
+
+val pureLoop = process_topdecs
   `fun pureLoop x = pureLoop x;
    val _ = pureLoop 1`
 
-val pureLoop2 =
+val pureLoop2 = process_topdecs
   `fun pureLoop x = pureLoop (x+1);
    val _ = pureLoop 1`
 
@@ -46,20 +240,6 @@ val (pureLoop_call_def,pureLoop_code_def) =
 val (pureLoop2_call_def,pureLoop2_code_def) =
   to_data pureLoop2 "pureLoop2"
 
-fun diff_code code1 code2 = let
-  val l1 = code1
-           |> dest_comb
-           |> snd
-           |> listSyntax.dest_list
-           |> fst;
-  val l2 = code2
-           |> dest_comb
-           |> snd
-           |> listSyntax.dest_list
-           |> fst;
-  val [(p1,p2)] = filter (not o (uncurry aconv)) (zip l1 l2)
-  in (p1,p2)
-  end
 
 val (p1,p2) = diff_code pureLoop_code_def pureLoop2_code_def
 
@@ -69,7 +249,10 @@ Theorem data_safe_pureLoop_code[local]:
   ∀s. s.safe_for_space ∧
       (∃x. lookup 0 s.locals = SOME x) ∧
       (lookup 249 s.code =
-         ^((rhs o concl o EVAL) ``lookup 249 pureLoop_data_code``))
+         ^((``lookup 249 pureLoop_data_code``
+           |> (REWRITE_CONV [pureLoop_code_def]
+               THENC EVAL)
+           |> rhs o concl)))
       ⇒ data_safe (evaluate ((SND o SND) ^p1, s))
 Proof
   measureInduct_on `^s.clock`
@@ -97,7 +280,10 @@ Theorem data_safe_pureLoop_code_shallow[local] =
 Theorem data_safe_pureLoop_code_timeout[local]:
   ∀s. (∃x. lookup 0 s.locals = SOME x) ∧
       (lookup 249 s.code =
-         ^((rhs o concl o EVAL) ``lookup 249 pureLoop_data_code``))
+         ^((``lookup 249 pureLoop_data_code``
+           |> (REWRITE_CONV [pureLoop_code_def]
+               THENC EVAL)
+           |> rhs o concl)))
       ⇒ ∃s'. evaluate ((SND o SND) ^p1, s) =
                (SOME (Rerr(Rabort Rtimeout_error)),s')
 Proof
@@ -117,106 +303,27 @@ QED
 Theorem data_safe_pureLoop_code_timeout_shallow[local] =
   data_safe_pureLoop_code_timeout |> simp_rule [to_shallow_thm,to_shallow_def]
 
-Overload monad_unitbind[local] = ``bind``
-Overload return[local] = ``return``
-
-val _ = monadsyntax.temp_add_monadsyntax()
-
 Theorem data_safe_pureLoop:
  ∀ffi coracle cc n. data_safe (evaluate (pureLoop_data_call,
                           initial_state ffi pureLoop_data_code
                                         coracle cc T 1000 32 n))
 Proof
-  (* Some tactics *)
-  let
-    val data_eval_step =
-      computeLib.RESTR_EVAL_TAC [ ``IS_NONE``
-                                , ``op_requires_names``
-                                , ``pureLoop_data_code``]
-      \\ fs [bvi_to_dataTheory.op_requires_names_eqn
-            , IS_NONE_DEF
-            , cut_state_opt_def
-            , get_vars_def
-            , lookup_def
-            , dataLangTheory.op_space_reset_def]
-    val strip_assign =
-      qmatch_goalsub_abbrev_tac `bind _ rest_ass _`
-      \\ ONCE_REWRITE_TAC [bind_def]
-      \\ rw [assign_def,data_safe_def]
-      \\ EVAL_TAC \\ rw [size_of_def,lookup_def,lookup_delete]
-      \\ ONCE_REWRITE_TAC [GSYM (EVAL ``pureLoop_data_code``)]
-      \\ Q.UNABBREV_TAC `rest_ass`
-      \\ fs [bvi_to_dataTheory.op_requires_names_eqn, dataLangTheory.op_space_reset_def]
-      \\ rw []
-    val open_call =
-      qmatch_goalsub_abbrev_tac `call _ (SOME nn)`
-      \\ qpat_assum `Abbrev (nn = _)` (fn ab =>
-         let val eq = CONV_RULE (REWR_CONV markerTheory.Abbrev_def) ab
-             val n  = rhs (concl eq)
-         in Q.UNABBREV_TAC `nn`
-         \\ rw [ call_def
-               , find_code_def
-               , push_env_def
-               , get_vars_def
-               , EVAL ``lookup ^n pureLoop_data_code``
-               , to_shallow_thm,to_shallow_def
-               , call_env_def,dec_clock_def
-               , cut_env_def,domain_def
-               , data_safe_def
-               , EMPTY_SUBSET]
-         end)
-    val close_call =
-      qmatch_goalsub_abbrev_tac `f (state_locals_fupd _ _)`
-      \\ qmatch_goalsub_abbrev_tac `f s`
-      \\ `data_safe (f s)` suffices_by
-         (EVERY_CASE_TAC \\ rw [data_safe_def]
-         \\ fs [data_safe_def,data_safe_move
-               ,set_var_safe_for_space]
-         \\ drule_then drule pop_env_safe_for_space
-         \\ fs [set_var_safe_for_space])
-      \\ Q.UNABBREV_TAC `f`
-      \\ Q.UNABBREV_TAC `s`
-    val make_call =
-      open_call \\ close_call
-    val open_tailcall =
-      qmatch_goalsub_abbrev_tac `tailcall (SOME nn)`
-      \\ qpat_assum `Abbrev (nn = _)` (fn ab =>
-         let val eq = CONV_RULE (REWR_CONV markerTheory.Abbrev_def) ab
-             val n  = rhs (concl eq)
-         in Q.UNABBREV_TAC `nn`
-         \\ rw [ tailcall_def
-               , find_code_def
-               , get_vars_def
-               , get_var_def
-               , lookup_def
-               , EVAL ``lookup ^n pureLoop_data_code``]
-         end)
-      \\ rw [ to_shallow_thm,to_shallow_def,call_env_def
-            , dec_clock_def,data_safe_def,size_of_def,lookup_def]
-    val close_tailcall =
-      ho_match_mp_tac data_safe_res
-      \\ reverse conj_tac >- (rw [] \\ pairarg_tac \\ rw [])
-      \\ rw []
-    val make_tailcall =
-      open_tailcall \\ close_tailcall
-    val strip_call =
-      qmatch_goalsub_abbrev_tac `bind _ rest_call _`
-      \\ ONCE_REWRITE_TAC [bind_def]
-      \\ open_call \\ rw [data_safe_def]
-    val make_if =
-      rw [if_var_def,data_safe_def,lookup_def]
-      \\ fs [ isBool_def
-            , backend_commonTheory.bool_to_tag_def
-            , backend_commonTheory.true_tag_def
-            , backend_commonTheory.false_tag_def]
-  (* Start *)
-  (* Turn into shallow embedding  *)
+ let
+  val code_lookup   = mk_code_lookup `pureLoop_data_code` pureLoop_code_def
+  val strip_assign  = mk_strip_assign code_lookup
+  val open_call     = mk_open_call code_lookup
+  val make_call     = mk_make_call open_call
+  val strip_call    = mk_strip_call open_call
+  val open_tailcall = mk_open_tailcall code_lookup
+  val make_tailcall = mk_make_tailcall open_tailcall
  in
+  (* Some tactics *)
  REWRITE_TAC [ definition "pureLoop_data_call_def"
-                , to_shallow_thm
-                , to_shallow_def]
+             , to_shallow_thm
+             , to_shallow_def
+             , initial_state_def]
+ \\ rpt strip_tac
   (* Make first call *)
- \\ rw [ initial_state_def ]
  \\ make_tailcall
  (* Bootcode *)
  \\ ntac 7 strip_assign
@@ -226,10 +333,11 @@ Proof
  \\ make_call
  \\ strip_call
  \\ ntac 9 strip_assign
- \\ data_eval_step
+ \\ make_if
  \\ UNABBREV_ALL_TAC
  (* Continues after call *)
- \\ ntac 50 strip_assign
+ \\ strip_makespace
+ \\ ntac 49 strip_assign
  (* Another tailcall *)
  \\ make_tailcall
  \\ strip_call
@@ -246,25 +354,561 @@ Proof
  \\ UNABBREV_ALL_TAC
  \\ ntac 3 strip_assign
  \\ make_tailcall
- \\ ntac 8 strip_assign
+ \\ strip_makespace
+ \\ ntac 7 strip_assign
  \\ make_tailcall
  \\ strip_assign
  (* Finally we reach our function call *)
  \\ ho_match_mp_tac data_safe_bind_error
  \\ open_call
- \\ rw [get_var_def,lookup_def,data_safe_def,to_shallow_def]
  \\ qmatch_goalsub_abbrev_tac `f (state_locals_fupd _ _)`
  \\ qmatch_goalsub_abbrev_tac `f s`
  \\ `∃s'. f s = (SOME (Rerr(Rabort Rtimeout_error)),s')`
     by (unabbrev_all_tac
        \\ ho_match_mp_tac data_safe_pureLoop_code_timeout_shallow
-       \\ rw [lookup_def,lookup_fromList]
-       \\ EVAL_TAC)
+       \\ rw [lookup_def,lookup_fromList,code_lookup])
  \\ `data_safe (f s)` suffices_by (rw [] \\ rfs [])
  \\ unabbrev_all_tac
  \\ ho_match_mp_tac data_safe_pureLoop_code_shallow
- \\ rw [lookup_def,lookup_fromList]
- \\ EVAL_TAC
+ \\ rw [lookup_def,lookup_fromList,code_lookup]
+ end
+QED
+
+(* ****************************** *)
+(* * condLoop (with mini-basis) * *)
+(* ****************************** *)
+
+(* A loop functions with a stopping condition *)
+
+val minus_prog = find_term (can (match_term ``Dlet _ (Pvar "-") _``)) whole_prog
+val equal_prog = find_term (can (match_term ``Dlet _ (Pvar "=") _``)) whole_prog
+
+val condLoop =
+  let val prog = process_topdecs
+        `fun condLoop x = if x = 0 then 0 else condLoop (x - 1);
+         val _ = condLoop 5`
+  in (rhs o concl o EVAL) ``[^minus_prog;^equal_prog] ++ ^prog``
+  end
+
+val condLoop2 =
+  let val prog = process_topdecs
+        `fun condLoop x = if x = 0 then 0 else condLoop (x - 2);
+         val _ = condLoop 5`
+  in (rhs o concl o EVAL) ``[^minus_prog;^equal_prog] ++ ^prog``
+  end
+
+val (condLoop_call_def,condLoop_code_def) =
+  to_data condLoop "condLoop"
+
+val (condLoop2_call_def,condLoop2_code_def) =
+  to_data condLoop2 "condLoop2"
+
+val (b1,b2) = diff_code condLoop_code_def condLoop2_code_def
+
+Theorem data_safe_basis_condLoop:
+ ∀ffi coracle cc n. data_safe (evaluate (condLoop_data_call,
+                          initial_state ffi condLoop_data_code
+                                        coracle cc T 10000 32 n))
+Proof
+ let
+  val code_lookup   = mk_code_lookup `condLoop_data_code` condLoop_code_def
+  val strip_assign  = mk_strip_assign code_lookup
+  val open_call     = mk_open_call code_lookup
+  val make_call     = mk_make_call open_call
+  val strip_call    = mk_strip_call open_call
+  val open_tailcall = mk_open_tailcall code_lookup
+  val make_tailcall = mk_make_tailcall open_tailcall
+ in
+ REWRITE_TAC [ definition "condLoop_data_call_def"
+             , to_shallow_thm
+             , to_shallow_def
+             , initial_state_def ]
+  (* Make first call *)
+ \\ rpt strip_tac
+ \\ make_tailcall
+ (* Bootcode *)
+ \\ ntac 7 strip_assign
+ (* Another call *)
+ \\ ho_match_mp_tac data_safe_bind_return
+ (* Yet another call *)
+ \\ make_call
+ \\ strip_call
+ \\ ntac 9 strip_assign
+ \\ make_if
+ \\ UNABBREV_ALL_TAC
+ (* Continues after call *)
+ \\ strip_makespace
+ \\ ntac 49 strip_assign
+ (* Another tailcall *)
+ \\ make_tailcall
+ \\ time (ntac 3
+    (strip_call
+    \\ ntac 9 strip_assign
+    \\ make_if
+    \\ UNABBREV_ALL_TAC))
+ \\ ntac 6 strip_assign
+ \\ open_tailcall
+ \\ time (ntac 3
+    (ntac 4 strip_assign
+    \\ make_if
+    \\ ntac 2 strip_assign
+    \\ open_tailcall))
+ \\ ntac 4 strip_assign
+ \\ make_if
+ \\ simp [code_lookup]
+ \\ IF_CASES_TAC >- simp [data_safe_def]
+ \\ close_tailcall
+ \\ REWRITE_TAC [ push_env_def , to_shallow_def , to_shallow_thm]
+ \\ eval_goalsub_tac ``state_locals_fupd _ _``
+ \\ ntac 3
+    (strip_makespace
+    \\ ntac 7 strip_assign
+    \\ make_tailcall)
+ \\ strip_assign
+ \\ strip_call
+ \\ ntac 5
+    (strip_assign
+    \\ make_if
+    \\ strip_assign
+    \\ strip_assign
+    \\ open_tailcall)
+ \\ strip_assign
+ \\ make_if
+ \\ strip_assign
+ \\ simp [return_def,lookup_def]
+ \\ Q.UNABBREV_TAC `rest_call`
+ \\ make_tailcall
+ \\ strip_assign
+ \\ simp [return_def,lookup_def]
+ \\ simp [data_safe_def]
+end
+QED
+
+(* ************************** *)
+(* * echo (with mini-basis) * *)
+(* ************************** *)
+
+val word8_mod =
+  find_term (can (match_term ``Dmod "Word8" _``)) whole_prog
+
+val word8_fromInt =
+  find_term (can (match_term ``Dlet _ (Pvar "fromInt") _``)) word8_mod
+
+val string_mod =
+  find_term (can (match_term ``Dmod "String" _``)) whole_prog
+
+val string_implode =
+  find_term (can (match_term ``Dlet _ (Pvar "implode") _``)) string_mod
+
+val word8array_mod =
+  find_term (can (match_term ``Dmod "Word8Array" _``)) whole_prog
+
+val word8array_array =
+  find_term (can (match_term ``Dlet _ (Pvar "array") _``)) word8array_mod
+
+val echo =
+  let val prog = process_topdecs `
+      fun put_char c = let
+        val s = String.implode [c]
+        val a = Word8Array.array 0 (Word8.fromInt 0)
+        val _ = #(put_char) s a
+        in () end;
+
+      fun printLoop c = (put_char c; printLoop c);
+
+      val _ = printLoop #"a"`
+  in (rhs o concl o EVAL) ``[Dmod "Word8"      [^word8_fromInt];
+                             Dmod "String"     [^string_implode];
+                             Dmod "Word8Array" [^word8array_array]
+                            ] ++ ^prog``
+  end
+
+val echo2 =
+  let val prog = process_topdecs `
+      fun put_char c = let
+        val a = Word8Array.array 0 (Word8.fromInt 0)
+        val s = String.implode [c]
+        val _ = #(put_char) s a
+        in () end;
+
+      fun printLoop c = (printLoop c; put_char c);
+
+      val _ = printLoop #"a"`
+  in (rhs o concl o EVAL) ``[Dmod "Word8"      [^word8_fromInt];
+                             Dmod "String"     [^string_implode];
+                             Dmod "Word8Array" [^word8array_array]
+                            ] ++ ^prog``
+  end
+
+val (echo_call_def,echo_code_def) =
+  to_data echo "echo"
+
+val (echo2_call_def,echo2_code_def) =
+  to_data echo2 "echo2"
+
+val f_diff = diff_codes echo_code_def echo2_code_def
+
+val (f11,f12) = hd f_diff
+val (f21,f22) = (hd o tl) f_diff
+
+Theorem data_safe_echo_code:
+  ∀s ts.
+   s.safe_for_space ∧
+   check_state s ∧
+   size_of_heap s ≤ s.limits.heap_limit ∧
+   (s.tstamps = SOME ts) ∧
+   (∃x. lookup 0 s.locals = SOME (Number 97)) ∧
+   (s.code = echo_data_code)
+   ⇒ data_safe (evaluate ((SND o SND) ^f21, s))
+Proof
+  let
+    val code_lookup   = mk_code_lookup `echo_data_code` echo_code_def
+    val strip_assign  = mk_strip_assign code_lookup
+    val open_call     = mk_open_call code_lookup
+    val make_call     = mk_make_call open_call
+    val strip_call    = mk_strip_call open_call
+    val open_tailcall = mk_open_tailcall code_lookup
+    val make_tailcall = mk_make_tailcall open_tailcall
+  in
+  measureInduct_on `^s.clock`
+  \\ fs [ to_shallow_thm
+        , to_shallow_def
+        , initial_state_def ]
+  \\ rw []
+  \\ strip_call
+  \\ qmatch_goalsub_abbrev_tac `f (state_locals_fupd _ _)`
+  \\ qmatch_goalsub_abbrev_tac `f s1`
+  \\ Q.UNABBREV_TAC `f`
+  \\ `check_state s1` by
+     by (Q.UNABBREV_TAC `s1`
+        \\ rw [check_state_def]
+        >- EVAL_TAC
+        >-
+
+
+  \\ strip_makespace
+  \\ ntac 6 strip_assign
+  \\ strip_call
+
+
+``lookup 61 echo_data_code``
+|> (REWRITE_CONV [echo_code_def] THENC EVAL)
+(* Finds out the length of the array *)
+
+``lookup 62 echo_data_code``
+|> (REWRITE_CONV [echo_code_def] THENC EVAL)
+(* Move the string into a byte array *)
+
+
+  \\ rw [ evaluate_def,get_var_def
+        , lookup_fromAList,get_vars_def
+        , find_code_def,call_env_def,data_safe_def]
+  \\ rw [lookup_fromList,dec_clock_def,lookup_fromAList,data_safe_def,cut_env_def]
+  \\ qmatch_goalsub_abbrev_tac `evaluate (_,s')`
+  \\ `s'.clock < s.clock` by rw [Abbr `s'`]
+
+
+  end
+QED
+
+
+Theorem data_safe_echo:
+ ∀ffi coracle cc n. data_safe (evaluate (echo_data_call,
+                          initial_state ffi echo_data_code
+                                        coracle cc T 1000 32 n))
+Proof
+ let
+  val code_lookup   = mk_code_lookup `echo_data_code` echo_code_def
+  val strip_assign  = mk_strip_assign code_lookup
+  val open_call     = mk_open_call code_lookup
+  val make_call     = mk_make_call open_call
+  val strip_call    = mk_strip_call open_call
+  val open_tailcall = mk_open_tailcall code_lookup
+  val make_tailcall = mk_make_tailcall open_tailcall
+ in
+ REWRITE_TAC [ definition "echo_data_call_def"
+             , to_shallow_thm
+             , to_shallow_def
+             , initial_state_def ]
+  (* Make first call *)
+ \\ rpt strip_tac
+ \\ make_tailcall
+ (* Bootcode *)
+ \\ ntac 7 strip_assign
+ \\ ho_match_mp_tac data_safe_bind_return
+ (* Yet another call *)
+ \\ make_call
+ \\ strip_call
+ \\ ntac 9 strip_assign
+ \\ make_if
+ \\ UNABBREV_ALL_TAC
+ (* Continues after call *)
+ \\ strip_makespace
+ \\ ntac 49 strip_assign
+ \\ make_tailcall
+ \\ ntac 4
+    (strip_call
+    \\ ntac 9 strip_assign
+    \\ make_if
+    \\ UNABBREV_ALL_TAC)
+  \\ strip_call
+  \\ ntac 9 strip_assign
+  \\ make_if
+  \\ ntac 6 strip_assign
+  \\ ntac 5
+     (open_tailcall
+     \\ ntac 4 strip_assign
+     \\ make_if
+     \\ ntac 2 strip_assign)
+  \\ open_tailcall
+  \\ ntac 4 strip_assign
+  \\ make_if
+  \\ Q.UNABBREV_TAC `rest_call`
+  \\ ntac 3 strip_assign
+  \\ make_tailcall
+  \\ ntac 5
+     (strip_makespace
+     \\ ntac 7 strip_assign
+     \\ make_tailcall)
+
+
+
+  \\ strip_assign
+  \\ strip_call
+  \\ strip_call
+
+
+
+  let val st =
+      (snd (top_goal()) |> find_term (can (match_term ``state_locals_fupd _ _``)))
+  in EVAL ``lookup 0 ^st.locals``
+  end
+
+f21
+
+
+
+
+
+
+
+
+val basis_echo =
+  let val prog = process_topdecs `
+      fun put_char c = let
+        val s = String.implode [c]
+        val a = Word8Array.array 0 (Word8.fromInt 0)
+        val _ = #(put_char) s a
+        in () end;
+
+      fun printLoop c = (put_char c; printLoop c);
+
+      val _ = printLoop #"a"`
+  in (rhs o concl o EVAL) ``^whole_prog ++ ^prog``
+  end
+
+val basis_echo2 =
+  let val prog = process_topdecs `
+      fun put_char c = let
+        val a = Word8Array.array 0 (Word8.fromInt 0)
+        val s = String.implode [c]
+        val _ = #(put_char) s a
+        in () end;
+
+      fun printLoop c = (printLoop c; put_char c);
+
+      val _ = printLoop #"a"`
+  in (rhs o concl o EVAL) ``^whole_prog ++ ^prog``
+  end
+
+val (basis_echo_call_def,basis_echo_code_def) =
+  to_data basis_echo "basis_echo"
+
+val (basis_echo2_call_def,basis_echo2_code_def) =
+  to_data basis_echo2 "basis_echo2"
+
+val bf_diff = diff_codes basis_echo_code_def basis_echo2_code_def
+
+val (bf11,bf12) = hd bf_diff
+val (bf21,bf22) = (hd o tl) bf_diff
+
+(* aconv (rand f12) (rand bf12) *)
+(* aconv (rand f21) (rand bf21) *)
+
+val basis_condLoop =
+  let val prog = process_topdecs
+        `fun basis_condLoop x = if x = 0 then 0 else basis_condLoop (x - 1);
+         val _ = basis_condLoop 5`
+  in (rhs o concl o EVAL) ``^whole_prog ++ ^prog``
+  end
+
+val basis_condLoop2 =
+  let val prog = process_topdecs
+        `fun basis_condLoop x = if x = 0 then 0 else basis_condLoop (x - 2);
+         val _ = basis_condLoop 5`
+  in (rhs o concl o EVAL) ``^whole_prog ++ ^prog``
+  end
+
+val (basis_condLoop_call_def,basis_condLoop_code_def) =
+  to_data basis_condLoop "basis_condLoop"
+
+val (basis_condLoop2_call_def,basis_condLoop2_code_def) =
+  to_data basis_condLoop2 "basis_condLoop2"
+
+val (c1,c2) = diff_code basis_condLoop_code_def basis_condLoop2_code_def
+
+Theorem data_safe_basis_condLoop:
+ ∀ffi coracle cc n. data_safe (evaluate (basis_condLoop_data_call,
+                          initial_state ffi basis_condLoop_data_code
+                                        coracle cc T 10000 32 n))
+Proof
+let
+  fun eval_goalsub_tac pat (asms,goal) =
+     let
+     val tm = goal |> find_term (can (match_term pat))
+     val th = EVAL tm
+     in PURE_ONCE_REWRITE_TAC [th] (asms,goal)
+     end
+  val code_lookup = EVERY_lookup
+      |> Q.ISPEC `basis_condLoop_data_code`
+      |> CONV_RULE ((RAND_CONV o RAND_CONV) (fn tm => basis_condLoop_code_def))
+      |> CONV_RULE (RAND_CONV EVAL)
+      |> SIMP_RULE (srw_ss()) []
+  val strip_makespace =
+      qmatch_goalsub_abbrev_tac `bind _ rest_mkspc _`
+      \\ REWRITE_TAC [ bind_def, makespace_def ]
+      \\ eval_goalsub_tac ``cut_env _ _`` \\ simp []
+      \\ eval_goalsub_tac ``state_locals_fupd _ _``
+      \\ Q.UNABBREV_TAC `rest_mkspc`
+  val strip_assign =
+      qmatch_goalsub_abbrev_tac `bind _ rest_ass _`
+      \\ REWRITE_TAC [ bind_def           , assign_def
+                     , op_space_reset_def , closLangTheory.op_case_def
+                     , cut_state_opt_def  , option_case_def
+                     , do_app_def         , data_spaceTheory.op_space_req_def
+                     , do_space_def       , closLangTheory.op_distinct
+                     , MEM                , IS_NONE_DEF
+                     , bvi_to_dataTheory.op_requires_names_eqn ]
+      \\ BETA_TAC
+      \\ TRY(eval_goalsub_tac ``cut_state _ _`` \\ simp [])
+      \\ TRY(eval_goalsub_tac ``get_vars    _ _`` \\ simp [])
+      \\ simp [ do_app_aux_def    , set_var_def    , lookup_def
+              , domain_IS_SOME    , code_lookup    , size_of_heap_def
+              , consume_space_def , with_fresh_ts_def
+              , backend_commonTheory.small_enough_int_def ]
+      \\ eval_goalsub_tac ``state_locals_fupd _ _``
+      \\ Q.UNABBREV_TAC `rest_ass`
+  val open_tailcall =
+      ASM_REWRITE_TAC [ tailcall_def , find_code_def
+                      , get_vars_def , get_var_def
+                      , lookup_def   , timeout_def ]
+      \\ simp [code_lookup,lookup_def]
+      \\ IF_CASES_TAC >- (simp [data_safe_def,size_of_def] \\ EVAL_TAC)
+      \\ REWRITE_TAC [ call_env_def   , dec_clock_def
+                     , to_shallow_thm , to_shallow_def ]
+      \\ eval_goalsub_tac ``state_locals_fupd _ _``
+    val close_tailcall =
+      ho_match_mp_tac data_safe_res
+      \\ reverse conj_tac >- (rw [] \\ pairarg_tac \\ rw [])
+    val make_tailcall =
+      open_tailcall \\ close_tailcall
+    val open_call =
+      ASM_REWRITE_TAC [ call_def     , find_code_def , push_env_def
+                      , get_vars_def , call_env_def  , dec_clock_def
+                      , cut_env_def  , domain_def    , data_safe_def
+                      , EMPTY_SUBSET , get_var_def ]
+      \\ simp [code_lookup,lookup_def]
+      \\ IF_CASES_TAC >- (simp [data_safe_def,size_of_def] \\ EVAL_TAC)
+      \\ REWRITE_TAC [ push_env_def , to_shallow_def , to_shallow_thm]
+      \\ eval_goalsub_tac ``state_locals_fupd _ _``
+    val close_call =
+      qmatch_goalsub_abbrev_tac `f (state_locals_fupd _ _)`
+      \\ qmatch_goalsub_abbrev_tac `f s`
+      \\ `data_safe (f s)` suffices_by
+         (EVERY_CASE_TAC \\ rw [data_safe_def]
+         \\ fs [data_safe_def,data_safe_move
+               ,set_var_safe_for_space]
+         \\ drule_then drule pop_env_safe_for_space
+         \\ fs [set_var_safe_for_space])
+      \\ Q.UNABBREV_TAC `f`
+      \\ Q.UNABBREV_TAC `s`
+    val make_call =
+      open_call \\ close_call
+    fun strip_call (asms,goal)=
+      let val free_names = map (fn tm => fst (dest_var tm)) (free_varsl (goal::asms))
+      fun next_name n name =
+          if mem name free_names
+          then next_name (n+1) (name ^ "_" ^ Int.toString (n+1))
+          else [QUOTE name]
+      qmatch_goalsub_abbrev_tac (`bind _ ` @ (next_name 0 "rest_call") @ ` _`)
+      \\ ONCE_REWRITE_TAC [bind_def]
+      \\ open_call \\ rw [data_safe_def]
+    val make_if =
+      simp [if_var_def,data_safe_def,lookup_def]
+      \\ REWRITE_TAC [ isBool_def
+                     , backend_commonTheory.bool_to_tag_def
+                     , backend_commonTheory.true_tag_def
+                     , backend_commonTheory.false_tag_def]
+      \\ simp [pop_env_def]
+      \\ eval_goalsub_tac ``state_locals_fupd _ _``
+  (* Start *)
+  (* Turn into shallow embedding  *)
+ in
+ REWRITE_TAC [ definition "basis_condLoop_data_call_def"
+             , to_shallow_thm
+             , to_shallow_def
+             , initial_state_def ]
+  (* Make first call *)
+ \\ rpt strip_tac
+ \\ make_tailcall
+ (* Bootcode *)
+ \\ ntac 7 strip_assign
+ (* Another call *)
+ \\ ho_match_mp_tac data_safe_bind_return
+ (* Yet another call *)
+ \\ make_call
+ \\ strip_call
+ \\ ntac 9 strip_assign
+ \\ make_if
+ \\ UNABBREV_ALL_TAC
+ (* Continues after call *)
+ \\ strip_makespace
+ \\ ntac 49 strip_assign
+ (* Another tailcall *)
+ \\ make_tailcall
+ \\ time (ntac 436
+    (strip_call
+    \\ ntac 9 strip_assign
+    \\ make_if
+    \\ UNABBREV_ALL_TAC))
+ \\ fs [NOT_LEQ]
+ \\ strip_call
+ \\ ntac 9 strip_assign
+ \\ make_if
+ \\ ntac 6 strip_assign
+ \\ open_tailcall
+ \\ qmatch_goalsub_abbrev_tac `f (_ (state_locals_fupd _ _))`
+ \\ `∀p. f (f p) = f p` by (Cases \\ Cases_on `q` \\ fs [Abbr `f`])
+ \\ Q.UNABBREV_TAC `f`
+ \\ time (ntac 437
+    (ntac 4 strip_assign
+    \\ make_if
+    \\ ntac 2 strip_assign
+    \\ open_tailcall
+    \\ ASM_REWRITE_TAC []))
+ (* HERE *)
+ \\ fs [NOT_LEQ]
+ \\ ntac 4 strip_assign
+ \\ make_if
+ \\ rw []
+ \\ Q.UNABBREV_TAC `rest_call`
+ \\ ntac 3 strip_assign
+ \\ make_tailcall
+ \\ ntac 17
+    (strip_makespace
+    \\ ntac 7 strip_assign
+    \\ make_tailcall)
+ \\ cheat
  end
 QED
 
